Define multiplication

Ray/Approx/Floating/Mul.lean
@@ -24,7 +24,7 @@ namespace Floating
 /-- The limit for our 64 bit → 128 bit multiplication -/
 def mul_n_max : ℕ := (2^63 - 1) ^ 2
 
-/-- Our 64 → 128 bit multiplication doesn't get too big -/
+/-- Our `64 → 128` bit integer multiplication doesn't get too big -/
 lemma mul_n_le {x y : Floating} (x0 : 0 ≤ x.val) (y0 : 0 ≤ y.val) :
     (mul128 x.n.n y.n.n).toNat ≤ mul_n_max := by
   rw [toNat_mul128, mul_n_max, pow_two]
@@ -36,19 +36,70 @@ lemma mul_n_le {x y : Floating} (x0 : 0 ≤ x.val) (y0 : 0 ≤ y.val) :
 ### The definition of multiplication
 -/
 
-/-- Normalize a 128-bit `n` into a 64-bit one, rounding and shifting as necessary. -/
+/-- Normalize a 128-bit `n` into a 64-bit one, rounding and shifting as necessary.
+    We also return how much we shifted left by. -/
 @[irreducible, inline] def mul_norm (n : UInt128) (up : Bool) : UInt64 × UInt64 :=
   let t := n.log2
+  let s := 126 - t
   -- Shift left to normalize
-  let z : UInt128 := n <<< (126 - t)
+  let z : UInt128 := n <<< s
   -- Round to a single word
-  let r : UInt64 := z.hi + bif z.lo != 0 && up then 1 else z.hi
-  (r, t)
+  let r : UInt64 := z.hi + bif z.lo != 0 && up then 1 else 0
+  -- If we round up too much, shift down by one
+  bif r == 2^63 then (2^62, s - 1) else (r, s)
 
 /-- `mul_norm` returns a normalized value -/
-lemma mul_norm_norm (n : UInt128) (up : Bool) (lo : n.toNat ≤ mul_n_max) :
+lemma mul_norm_norm (n : UInt128) (up : Bool) (n0 : n ≠ 0) (lo : n.toNat ≤ mul_n_max) :
     (mul_norm n up).1.toNat ∈ Ico (2^62) (2^63) := by
-  sorry
+  rw [mul_norm]
+  generalize ht : n.log2 = t
+  generalize hs : 126 - t = s
+  generalize hz : n <<< s = z
+  generalize hb : (bif z.lo != 0 && up then (1 : UInt64) else 0) = b
+  generalize hr : z.hi + b = r
+  generalize hp : (bif r == 2^63 then (2^62, s - 1) else (r, s)) = p
+  simp only [hz, Bool.and_eq_true, bne_iff_ne, ne_eq, hr, mem_Ico, hb, hs, hp]
+  simp only [UInt64.eq_iff_toNat_eq, UInt128.toNat_log2, UInt128.eq_iff_toNat_eq,
+    UInt128.toNat_shiftLeft', UInt64.toNat_add, UInt64.size_eq_pow, bif_eq_if,
+    apply_ite (f := fun x : UInt64 ↦ x.toNat), UInt64.toNat_zero,
+    UInt64.toNat_one, beq_iff_eq, up63] at ht hz hb hr hs hp
+  rw [UInt128.ne_zero_iff] at n0
+  have t_le : t.toNat ≤ 126 := by
+    rw [←ht, ←Nat.lt_succ_iff, Nat.log2_lt n0]; exact lt_of_le_of_lt lo (by norm_num [mul_n_max])
+  have t_le' : t ≤ 126 := by simp only [UInt64.le_iff_toNat_le, u126, t_le]
+  simp only [UInt64.toNat_sub t_le', u126] at hs
+  have s_lt : s.toNat < 128 := by rw [←hs]; omega
+  have nt' : n.toNat * 2^s.toNat < 2^127 := by
+    refine lt_of_lt_of_le (Nat.mul_lt_mul_of_pos_right Nat.lt_log2_self (by positivity)) ?_
+    simp only [ht, ← pow_add, ←hs]
+    exact pow_le_pow_right (by norm_num) (by omega)
+  have nt : n.toNat * 2^s.toNat < 2^128 := lt_trans nt' (by norm_num)
+  have b1 : b.toNat ≤ 1 := by rw [←hb]; split_ifs; repeat norm_num
+  simp only [UInt64.toNat_sub t_le', u126, Nat.mod_eq_of_lt s_lt, Nat.mod_eq_of_lt nt] at hz
+  have z_lt : z.toNat < 2^127 := by rwa [←hz]
+  have r_le : z.hi.toNat + b.toNat ≤ 2^63 := by
+    rw [UInt128.toNat_def] at z_lt
+    contrapose z_lt; simp only [not_le, not_lt] at z_lt ⊢
+    have zh63 : 2^63 ≤ z.hi.toNat := by omega
+    exact le_trans (le_trans (by norm_num) (Nat.mul_le_mul_right _ zh63)) (Nat.le_add_right _ _)
+  rw [Nat.mod_eq_of_lt (lt_of_le_of_lt r_le (by norm_num))] at hr
+  rw [hr] at r_le
+  have le_z : 2^126 ≤ z.toNat := by
+    rw [←hz, ←hs, ←ht]
+    refine le_trans ?_ (Nat.mul_le_mul_right _ (Nat.log2_self_le n0))
+    rw [←pow_add]
+    exact pow_le_pow_right (by norm_num) (by omega)
+  have le_r : 2^62 ≤ r.toNat := by
+    rw [←hr]
+    refine le_trans ?_ (Nat.le_add_right _ _)
+    rw [UInt128.toNat_def] at le_z
+    have zl := z.lo.toNat_lt
+    norm_num only at le_z zl ⊢
+    omega
+  rw [←hp]
+  split_ifs with r_eq
+  · rw [up62]; decide
+  · simp only [ite_false, le_r, r_le.lt_of_ne r_eq, and_self]
 
 /-- Build a `Floating` with value `n * 2^s`, rounding if necessary -/
 @[irreducible, inline] def mul_finish (n : UInt64) (s : UInt128) (up : Bool)
@@ -86,9 +137,10 @@ lemma mul_norm_norm (n : UInt128) (up : Bool) (lo : n.toNat ≤ mul_n_max) :
 @[irreducible, inline] def mul_of_pos (x y : Floating) (up : Bool)
     (x0 : 0 ≤ x.val) (y0 : 0 ≤ y.val) : Floating :=
   let z := mul128 x.n.n y.n.n  -- `z * 2^(x.s + y.s - 2^64)`.
+  if z0 : z = 0 then 0 else
   let n := mul_norm z up  -- `n.1 * 2^(x.s + y.s + n.2 - 62 - 2^64)`
   let e := mul_exponent x.s y.s n.2  -- `n.1 * 2^e`
-  mul_finish n.1 e up (mul_norm_norm z up (mul_n_le x0 y0))
+  mul_finish n.1 e up (mul_norm_norm z up z0 (mul_n_le x0 y0))
 
 /-- Floating point multiply -/
 @[irreducible] def mul (x y : Floating) (up : Bool) : Floating :=
